finishes basic props of LR, but with dirty proofs

theories/LogicalRelation.v
@@ -101,10 +101,28 @@ Definition ϵPi i j S1 S2 (ϵS : TmRel) T1 T2 (ϵT : forall s1 s2, ϵS s1 s2 -> 
         ∙ ⊢< Ru i j > f1 ≡ f2 : Pi i j S1 T1 /\
         forall s1 s2 (ϵs : ϵS s1 s2), ϵT s1 s2 ϵs (app i j S1 T1 f1 s1) (app i j S2 T2 f2 s2).
 
-(* TODO replace conv by reduction *)
-
+Definition same_rel (R1 R2 : term -> term -> Prop) := forall t u, R1 t u <-> R2 t u.
 
 Notation "R1 <~> R2" :=  (forall t u, R1 t u <-> R2 t u) (at level 50, R2 at next level).
+
+Instance same_relation_subst :
+  Proper (same_rel ==> pointwise_relation _ (pointwise_relation _ iff))
+         (fun R x y => R x y).
+Proof.
+  intros R R' H x y.
+  split; intros; unfold same_rel in H; rewrite H in *; eauto.
+Qed.
+
+(* Notation "R1 <~> R2" :=  (forall t u, R1 t u <-> R2 t u) (at level 50, R2 at next level). *)
+
+(* Add Parametric Morphism : same_rel
+  with signature ((pointwise_relation _ eq) ==> (pointwise_relation _ eq) ==> iff)
+  as Phi_mor.
+Proof.
+  intros f₁ f₂ Hf g₁ g₂ Hg.
+  split; eauto using refines_preserves_eq.
+  apply refines_preserves_eq; apply pointwise_symmetric; eauto using eq_sym.
+Qed. *)
 
 Inductive LRTy : forall (k : nat) (rec : forall j, j ◃ (ty k) -> LogRel), LogRel :=
 | LRTy_nat A1 A2 rec R : 
@@ -333,17 +351,85 @@ Proof.
       intros. eapply redd_whnf_to_conv in A1_red_pi, A2_red_pi.
       eapply conv_trans. eapply A1_red_pi. eapply conv_trans. 2:(eapply conv_sym; eapply A2_red_pi).
       eapply conv_pi; eauto.
-      intros. rewrite H in H2. destruct H2. eauto using conv_conv, redd_whnf_to_conv, conv_sym.
+      intros. apply H in H2. destruct H2. eauto using conv_conv, redd_whnf_to_conv, conv_sym.
 Qed.
 
 
-Lemma conv_aux i j s1 s2 S1 T1 T2 : 
+(* we split the result in two, so we can use eauto with it *)
+Corollary LR_escape_ty {l A B R} : 
+    LR l A B R -> ∙ ⊢< Ax l > A ≡ B : Sort l.
+Proof.
+    intros. eapply LR_escape in H as (H1 & H2). eauto.
+Qed.
+
+Corollary LR_escape_tm  {l A B R t u }: 
+    LR l A B R -> R t u -> ∙ ⊢< l > t ≡ u : A.
+Proof.
+    intros. eapply LR_escape in H as (H1 & H2). eauto.
+Qed.
+
+Lemma conv_aux {i j s1 s2 S1 T1 T2} : 
     ∙ ⊢< i > s1 ≡ s2 : S1 -> ∙,, (i, S1) ⊢< Ax j > T1 ≡ T2 : Sort j -> ∙ ⊢< Ax j > T1 <[ s1 ..] ≡ T2 <[ s2.. ] : Sort j.
 Proof.
     intros. assert (Sort j = Sort j <[ s1 ..]). ssimpl; eauto.
     rewrite H1. eapply subst. eapply (conv_scons _ _ _ ∙  i S1). ssimpl. eapply refl_subst. eapply subst_id. eauto using ctx_typing.
     ssimpl. eauto. eauto.
 Qed.
+
+Section helper_aconv_app.
+    Context i j s1 s2 S1 S2 T1 T2 ϵS
+    (S1_conv_S2 : ∙ ⊢< Ax i > S1 ≡ S2 : Sort i)
+    (T1_conv_T2 : ∙,, (i, S1) ⊢< Ax j > T1 ≡ T2 : Sort j)
+    (LR_S : LR i S1 S2 ϵS) (ϵs : ϵS s1 s2).
+
+Ltac helper_solve :=     
+    eapply LR_escape_tm in ϵs; eauto;
+    eapply aconv_app; eauto using conv_sym, conv_ty_in_ctx_conv, refl_ty, validity_conv_left, LR_escape_ty, type_conv.
+
+Lemma aux1 t1 t2 (t1_aconv_t2 : ∙ ⊢< Ru i j > t1 ~ t2 : Pi i j S1 T1) :
+    ∙ ⊢< j > app i j S1 T1 t1 s1 ~ app i j S1 T1 t2 s1 : T1 <[ s1..].
+Proof.
+    helper_solve.
+Qed.
+
+Lemma aux2 t1 t2 (t1_aconv_t2 : ∙ ⊢< Ru i j > t1 ~ t2 : Pi i j S2 T2):
+    ∙ ⊢< j > app i j S2 T2 t1 s1 ~ app i j S1 T1 t2 s1 : T2 <[ s1..].
+Proof.
+    helper_solve.
+Qed.
+
+Lemma aux3 t1 t2 (t1_aconv_t2 : ∙ ⊢< Ru i j > t1 ~ t2 : Pi i j S1 T1):
+    ∙ ⊢< j > app i j S1 T1 t1 s2 ~ app i j S1 T1 t2 s2 : T1 <[ s2..].
+Proof.
+    helper_solve.
+Qed.
+
+Lemma aux4 t1 t2 (t1_aconv_t2 : ∙ ⊢< Ru i j > t1 ~ t2 : Pi i j S2 T2):
+    ∙ ⊢< j > app i j S2 T2 t1 s2 ~ app i j S1 T1 t2 s2 : T2 <[ s2..].
+Proof.
+    helper_solve.
+Qed.  
+
+Lemma aux5 t1 t2 (t1_aconv_t2 : ∙ ⊢< Ru i j > t1 ~ t2 : Pi i j S1 T1):
+    ∙ ⊢< j > app i j S1 T1 t1 s1 ~ app i j S2 T2 t2 s1 : T1 <[ s1..].
+Proof.
+    helper_solve.
+Qed.  
+
+Lemma aux6  t1 t2 (t1_aconv_t2 : ∙ ⊢< Ru i j > t1 ~ t2 : Pi i j S2 T2):
+    ∙ ⊢< j > app i j S2 T2 t1 s1 ~ app i j S2 T2 t2 s1 : T2 <[ s1..].
+Proof.
+    helper_solve.
+Qed.
+
+Lemma aux7 t1 t2 (t1_aconv_t2 : ∙ ⊢< Ru i j > t1 ~ t2 : Pi i j S1 T1):
+    ∙ ⊢< j > app i j S1 T1 t1 s2 ~ app i j S2 T2 t2 s2 : T1 <[ s2..].
+Proof.
+    helper_solve.
+Qed.
+
+End helper_aconv_app.
+
 
 Lemma LR_erasure l A B R : 
     LR l A B R -> 
@@ -387,24 +473,11 @@ Proof.
         + rewrite H in *. destruct H4. apply redd_whnf_to_conv in A1_red_pi as A1_conv_pi. split.
             ++ eauto 8 using sim_to_conv, conv_trans, conv_sym, conv_conv.
             ++ intros.
-               destruct (H1 s1 s2 ϵs). 
-               destruct (LR_escape _ _ _ _ (LR_T s1 s2 ϵs)) as (T1_s1_conv_T2_s2 & K). 
-               destruct (LR_escape _ _ _ _ LR_S). apply H9 in ϵs as s1_conv_s2.
-               apply validity_conv_left in s1_conv_s2 as s1_Wt. 
-               apply validity_conv_right in s1_conv_s2 as s2_Wt.
-               eapply type_conv in s2_Wt; eauto.
-               eapply H7; eauto.
-               eapply redd_whnf_to_conv in A2_red_pi as pi2.
-               eapply validity_conv_right in pi2. 
-               eapply type_inv_pi in pi2 as (S2_Wt & T2_Wt). 
-                eapply redd_whnf_to_conv in A1_red_pi as pi1.
-               eapply validity_conv_right in pi1. 
-               eapply type_inv_pi in pi1 as (S1_Wt & T1_Wt).
-               eapply aconv_app; eauto using validity_conv_left, refl_ty.
-               eapply aconv_conv; eauto.
-               eapply aconv_conv. 2: eauto using conv_aux, conv_sym.
-               eapply aconv_app; eauto 7 using refl_ty, validity_conv_right, conv_ty_in_ctx_conv. 
-               eapply aconv_conv; eauto. eapply conv_trans; eauto. eauto using conv_pi.
+               destruct (H1 s1 s2 ϵs). eapply H7; eauto.
+               +++ eapply aconv_app; eauto 7 using validity_conv_left, refl_ty, LR_escape_tm, redd_whnf_to_conv, aconv_conv.
+               +++ eapply aconv_conv; eauto using conv_aux, conv_sym, LR_escape_tm.
+                   eapply aconv_app; eauto 9 using validity_conv_right, refl_ty, conv_ty_in_ctx_ty, LR_escape_tm, LR_escape_ty, type_conv.
+                   eauto using aconv_conv, redd_whnf_to_conv, conv_sym, conv_trans, conv_pi.
 Qed.
 
 Definition LR_inv_type l A1 A2 A1' R (A1_redd_A1' : ∙ ⊢< Ax l > A1 -->>! A1' : Sort l) : Prop :=
@@ -462,33 +535,26 @@ Proof.
     - intros. eapply (LR_inv A1_red_U) in H1. destruct H1 as (_ & _ & _ & H'). rewrite H0. rewrite H'. split; eauto.
     - intros. eapply (LR_inv A1_red_pi) in H2. 
       destruct H2 as (S2' & T2' & ϵS' & ϵT' & l_eq & A1_red' & A2_red' & S_eq & T_eq & LR_S' & LR_T' & R_eq).
-      assert (ϵS <~> ϵS') by eauto. rewrite R_eq. 
-      intros. split. 
-      intro.
-      unfold ϵPi. rewrite H in H3. destruct H3. split; auto.
-      intros. assert (forall s1 s2 ϵs, ϵT s1 s2 (proj2 (H2 s1 s2) ϵs) <~> ϵT' s1 s2 ϵs).
-      intros. eapply H1. eauto. 
-      apply H5.
-      assert (ϵT s1 s2 (proj2 (H2 s1 s2) ϵs) (app i (ty k) S1 T1 t1 s1) (app i (ty k) S2 T2 t2 s2)).
-      apply H4.
-      destruct (LR_erasure _ _ _ _ (LR_T s1 s2 (proj2 (H2 s1 s2) ϵs))).
-      apply LR_escape in LR_S' as temp. pose proof ϵs as s1_conv_s2. apply (proj2 temp) in s1_conv_s2. clear temp.
-      eapply H8; eauto. 
-      eapply aconv_app; eauto using refl_ty, validity_conv_left, aconv_refl.
-      eapply aconv_conv. 2: eapply conv_aux. 2,3:eapply conv_sym. 2:eauto. 2: eapply T1_eq_T2.
-      eapply aconv_app; eauto 8 using refl_ty, validity_conv_left, aconv_refl, conv_trans, conv_sym, validity_conv_right, type_conv, conv_ty_in_ctx_conv.
-      admit.
-      intro. rewrite H.
-      unfold ϵPi. destruct H3. split; auto.
-      intros. assert (forall s1 s2 ϵs, ϵT s1 s2 ϵs <~> ϵT' s1 s2 (proj1 (H2 s1 s2) ϵs)).
-      intros. eapply H1. eauto. 
-      apply H5.
-      assert (ϵT' s1 s2 (proj1 (H2 s1 s2) ϵs) (app i (ty k) S1 T1 t1 s1) (app i (ty k) S2' T2' t2 s2)).
-      apply H4.
-      destruct (LR_erasure _ _ _ _ (LR_T' s1 s2 (proj1 (H2 s1 s2) ϵs))).
-      eapply H8; eauto. admit. admit.
-Admitted.
-
+      assert (ϵS <~> ϵS') by eauto. 
+      rewrite R_eq, H. 
+      split.
+      + intros. destruct H3. split. eauto. intros.
+        assert (forall s1 s2 ϵs, ϵT s1 s2 (proj2 (H2 s1 s2) ϵs) <~> ϵT' s1 s2 ϵs).
+            { intros. eapply H1. eauto. }
+        eapply H5. eapply LR_erasure; eauto. 
+        ++ rewrite <- H2 in ϵs. unshelve eauto using aconv_refl, type_app, LR_escape_tm, validity_conv_left; eauto.
+        ++ eapply aconv_conv; eauto using conv_aux, LR_escape_tm, conv_sym.
+           eapply sim_sym. eapply aconv_app; eauto using conv_trans, conv_sym, conv_ty_in_ctx_conv, LR_escape_tm, LR_escape_ty, type_conv, validity_conv_right.
+           eapply aconv_conv; eauto using aconv_refl, validity_conv_right, conv_pi, conv_sym, conv_trans, conv_ty_in_ctx_conv.
+      + intros. destruct H3. split. eauto. intros.
+        assert (forall s1 s2 ϵs, ϵT' s1 s2 (proj1 (H2 s1 s2) ϵs) <~> ϵT s1 s2 ϵs).
+            { intros. symmetry. eapply H1. eauto. }
+        eapply H5.  eapply LR_erasure; eauto.
+        ++ rewrite H2 in ϵs. unshelve eauto using aconv_refl, type_app, LR_escape_tm, validity_conv_left; eauto.
+        ++ eapply aconv_conv; eauto using conv_aux, LR_escape_tm, conv_sym.
+           eapply aconv_app; eauto using conv_trans, conv_sym, conv_ty_in_ctx_conv, LR_escape_tm, LR_escape_ty, type_conv, validity_conv_right.
+           eapply aconv_conv; eauto using aconv_refl, validity_conv_right, conv_pi, conv_sym, conv_trans, conv_ty_in_ctx_conv.
+Qed.
 
 Definition PER {A} (R:A -> A -> Prop) := 
     (forall t u, R t u -> R u t) /\ (forall t u v, R t v -> R v u -> R t u).
@@ -511,121 +577,196 @@ Proof.
     - eapply LR_pi; eauto. intros. rewrite <- H2. eauto.
 Qed. 
 
+Lemma helper_ϵT_irrel {ϵS : TmRel} 
+    (ϵT : forall s1 s2, ϵS s1 s2 -> TmRel) {s1 s2} {ϵs ϵs'} {t u}: 
+    ϵT s1 s2 ϵs t u -> ϵT s1 s2 ϵs' t u.
+Proof.
+    intros. assert (ϵs = ϵs') by eauto using proof_irrel. subst. eauto.
+Qed.
 
-Lemma aux' l A B R :
+Lemma LR_basic_props l A B R :
     LR l A B R ->
     PER R /\
     LR l B A R /\ 
-    (forall R' C, LR l B C R' -> LR l A C R' /\ R <~> R') /\
-    (forall R' C, LR l C A R' -> LR l C B R' /\ R <~> R').
+    (forall R' C, LR l B C R' -> LR l A C R' /\ R <~> R').
 Proof.
     generalize l A B R. clear l A B R.
     refine (LR_ind _ _ _ _ _).
-    - intros. split. 2:split. 3:split.
+    - intros. split. 2:split.
       + destruct p. split; intros; rewrite H0 in *; eauto using conv_sym, conv_trans.
       + rewrite LR_prop_eq. destruct p. split; eauto using conv_sym. intros. 
         rewrite (H0 t u). split; intros; eauto using conv_conv, conv_sym.
       + intros. rewrite LR_prop_eq in *. destruct H, p. split. split; eauto using conv_trans.
         intros. rewrite (H0 t u). split; intros; eauto using conv_conv, conv_sym.
         intros. rewrite (H2 t u). rewrite (H0 t u).  split; intros; eauto using conv_conv, conv_sym.
-      + intros. rewrite LR_prop_eq in *. destruct H, p. split. split; eauto using conv_trans.
-        intros. rewrite (H2 t u). rewrite (H0 t u).  split; intros; eauto using conv_conv, conv_sym.
-    - intros. split. 2:split. 3:split.
+    - intros. split. 2:split.
       + split; intros; rewrite H in *. 
         destruct H0 as (k & H1 & H2). eexists. split; eauto.
         destruct H0 as (k & t_red & v_red). destruct H1 as (k' & v_red' & u_red).
-        exists k. split. eauto. admit.
+        exists k. split. eauto. 
+        eapply redd_whnf_det in v_red'. 2:eapply v_red. rewrite v_red'. eauto.
       + eapply LR_nat; eauto.
       + intros. unshelve eapply LR_inv in H0. shelve. eapply A2_red_nat. 
         destruct H0 as (_ & _ & C_red & R'_iff_nat). 
         split. eauto using LR_nat. intros. rewrite H. rewrite R'_iff_nat. split; auto.
-      + intros. admit.
-    - intros. split. 2:split. 3:split.
+    - intros. split. 2:split.
       + split; intros; rewrite H0 in *. destruct H1. destruct (H _ _ _ H1) as (_ & H' & _). eexists. eauto.
-        destruct H1. destruct H2. destruct (H _ _ _ H1) as (_ & _  & H' & H'').
+        destruct H1. destruct H2. destruct (H _ _ _ H1) as (_ & _  & H').
         destruct (H' _ _ H2). eexists. eauto.
       + eapply LR_U; eauto. 
       + intros. pose proof H1 as H1'. unshelve eapply LR_inv in H1. shelve. eauto. destruct H1 as (_ & _ & C_red & H').
         split. eapply LR_U; eauto.
         intros; split; rewrite H'; rewrite H0; intros; eauto.
-      + admit.
     - intros. 
-      destruct H0 as (PER_ϵS & LR_S_sym & LR_S_trans_left & LR_S_trans_right).
+      destruct H0 as (PER_ϵS & LR_S_sym & LR_S_trans).
       pose proof PER_ϵS as PER_ϵS'.
       destruct PER_ϵS as (ϵS_sym & ϵS_trans). rename PER_ϵS' into PER_ϵS.
       assert (forall s1 s2 ϵs, 
         ϵT s1 s2 ϵs <~> ϵT s2 s1 (ϵS_sym _ _ ϵs) /\ ϵT s1 s2 ϵs <~> ϵT s2 s2 (PER_refl PER_ϵS (ϵS_sym _ _ ϵs))).
       { intros. pose (ϵs' := ϵS_sym _ _ ϵs). pose (ϵs'' := PER_refl PER_ϵS ϵs').
-        pose (LR_T_s1_s2 := LR_T _ _ ϵs).
-        pose (LR_T_s2_s1 := LR_T _ _ ϵs').
-        pose (LR_T_s2_s2 := LR_T _ _ ϵs'').
-        destruct (H1 _ _ ϵs) as (_ & LR_T_s1_s2' & _).
-        destruct (H1 _ _ ϵs') as (_ & LR_T_s2_s1' & _).
-        destruct (H1 _ _ ϵs'') as (_ & _ & LR_T_trans_left & LR_T_trans_right).
-        eapply LR_T_trans_left in LR_T_s1_s2' as (_ & HA).
-        eapply LR_T_trans_right in LR_T_s2_s1' as (_ & HB).
-        unfold ϵs' in HB.
-        split.
-        + split; intros; rewrite <- HA in *; rewrite <- HB in *; eauto.
-        + unfold ϵs'', ϵs' in *. symmetry. rewrite HA. split; intros; eauto. }
-      split. 2:split. 3:split.
+        destruct (H1 _ _ ϵs) as (_ & LR_T_s1_s2 & _).
+        destruct (H1 _ _ ϵs'') as (_ & LR_T_s2_s2 & _).
+        pose (HA' := LR_T _ _ ϵs''). pose (HB' := LR_T _ _ ϵs').
+        assert (ϵT s2 s1 ϵs' <~> ϵT s2 s2 ϵs'') as ϵT_21_22 
+            by eauto using LR_irrel.
+        assert (ϵT s1 s2 ϵs <~> ϵT s2 s2 ϵs'') as ϵT_12_22
+            by eauto using LR_irrel.
+        unfold ϵs' in ϵT_21_22.
+        split. 
+        + split; rewrite ϵT_21_22; rewrite ϵT_12_22; eauto.
+        + unfold ϵs'', ϵs' in ϵT_12_22. eauto. }
+      split. 2:split.
       + split; intros; rewrite H in *. 
         ++ destruct H2. split; eauto using conv_sym.
            intros. destruct (H1 _ _ ϵs) as ((ϵT_sym & ϵT_trans) & _). eapply ϵT_sym.
-           eapply (proj1 (H0 _ _ _)). pose (H3' := H3 _ _ (ϵS_sym _ _ ϵs)). admit.
+           eapply (proj1 (H0 _ _ _)). 
+           eapply LR_erasure; eauto. 
+           +++ eapply aconv_app; eauto using aconv_refl, validity_conv_left, LR_escape_tm, validity_conv_right.
+           +++ eapply aconv_conv; eauto using conv_aux, conv_sym, LR_escape_tm.
+               eapply aconv_app; eauto using LR_escape_tm, validity_conv_right, conv_sym, conv_ty_in_ctx_conv.
+               eapply aconv_conv; eauto using aconv_refl, validity_conv_right, conv_pi.
         ++ destruct H2, H3. split; eauto using conv_trans.
            intros. destruct (H1 _ _ ϵs) as ((ϵT_sym & ϵT_trans) & _). eapply ϵT_trans.
-           eapply H4. eapply (proj2 (H0 _ _ _)). pose (H5' := H5 _ _ (PER_refl PER_ϵS (ϵS_sym s1 s2 ϵs))). admit.
-      + eapply LR_pi; eauto using conv_sym, conv_ty_in_ctx_conv. intros.
-        destruct (H1 _ _ (ϵS_sym _ _ ϵs)) as (_ & H3' & _).
-        eapply LR_iff_rel. eapply (proj1 (H0 _ _ _)). eapply H3'.
-        split; intros; rewrite H in *. destruct H2. split. admit.
-        intros. pose (H3' := H3 _ _ (ϵS_sym s2 s1 (ϵS_sym s1 s2 ϵs))). admit.
-        destruct H2. split. admit.
-        intros. pose (H3' := H3 _ _ ϵs). admit.
-      + intros. pose proof H2 as H2'. unshelve eapply LR_inv in H2. shelve. eauto. 
+           eapply H4. clear H4. eapply (proj2 (H0 _ _ _)). 
+           eapply LR_erasure; eauto. 
+           +++ eapply aconv_app; eauto using aconv_refl, validity_conv_left, LR_escape_tm, validity_conv_right.
+           +++ eapply aconv_conv.
+               eapply aconv_app; eauto using LR_escape_tm, validity_conv_left, refl_ty, conv_sym, conv_ty_in_ctx_conv.
+               eapply aconv_conv; eauto using aconv_refl, validity_conv_right, conv_pi.
+               eauto 6 using conv_aux, conv_sym, LR_escape_tm, validity_conv_right, refl_ty.
+      + eapply LR_pi; eauto using conv_sym, conv_ty_in_ctx_conv. 
+        ++ intros.
+            destruct (H1 _ _ (ϵS_sym _ _ ϵs)) as (_ & H3' & _).
+            eapply LR_iff_rel.  eapply (proj1 (H0 _ _ _)). eapply H3'.
+        ++ split; intros; rewrite H in *. 
+            +++ destruct H2. split. 
+                eauto using conv_conv, conv_pi. 
+                intros. eapply LR_erasure; eauto. 
+                ++++ eapply aconv_app; eauto using aconv_refl, validity_conv_left, LR_escape_tm, validity_conv_right.
+                ++++ eapply aconv_conv. 
+                     eapply aconv_app; eauto using aconv_refl, validity_conv_left, LR_escape_tm, validity_conv_right, conv_ty_in_ctx_conv, conv_sym.
+                     eapply aconv_conv; eauto using validity_conv_right, aconv_refl, conv_pi. 
+                     eauto using conv_sym, LR_escape_tm, conv_aux.
+            +++ destruct H2. split. 
+                eauto using conv_conv, conv_pi, conv_sym.
+                intros. 
+                eapply (helper_ϵT_irrel ϵT).
+                eapply LR_erasure; eauto.
+                ++++ eapply aconv_conv.
+                     eapply aconv_app; eauto using conv_sym, conv_ty_in_ctx_conv, validity_conv_left, aconv_refl, LR_escape_tm, type_conv.
+                     eauto 6 using conv_sym, conv_aux, LR_escape_tm, validity_conv_left, type_conv. Unshelve. eauto.
+                ++++ eapply aconv_conv.
+                     eapply aconv_app; eauto using validity_conv_right, type_conv, conv_sym, LR_escape_tm. 
+                     eapply aconv_conv; eauto using validity_conv_right, aconv_refl, conv_pi, conv_sym, conv_ty_in_ctx_conv.
+                     eauto 7 using conv_aux, LR_escape_tm, conv_sym, validity_conv_left, refl_ty.
+      + intros. 
+      
+        pose proof H2 as H2'. unshelve eapply LR_inv in H2. shelve. eauto. 
         destruct H2 as (S' & T' & ϵS' & ϵT' & _ & _ & C_red & S2_eq_S' & T2_eq_T' & LR_S' & LR_T' & R'_iff).
-        pose proof (ϵS_iff_ϵS' := LR_irrel _ _ _ _ _ _ LR_S_sym LR_S').
-        assert (forall s1 s2, ϵS' s1 s2 -> ϵS' s2 s1) as ϵS'_sym. intros. rewrite <- ϵS_iff_ϵS' in *. eauto.
-        (* eassert (∀ (s1 s2 : term) (ϵs : ϵS' s1 s2), LR (ty k) (T1 <[ s1..]) (T' <[ s2..]) _).
-        intros. *)
 
-        (* apply ϵS_sym in ϵs as ϵs'. *)
-        eassert (forall s1 s2 (ϵs : ϵS s1 s2), LR (ty k) (T2 <[ s2..]) (T' <[ s1..]) (ϵT' s2 s1 _)). 
-        intros. pose (ϵs' := proj1 (ϵS_iff_ϵS' _ _) (ϵS_sym _ _ ϵs)).  eapply (LR_T' _ _ ϵs').
-        (* epose proof (ϵT_iff_ϵT' := fun s1 s2 (ϵs : ϵS s1 s2) => LR_irrel _ _ _ _ _ _ (proj1 (proj2 (H1 _ _ ϵs))) _. 
-        shelve. shelve. eapply (LR_T'  _ _ (ϵ)
-        assert (ϵS <~> ϵS'). split;  *)
+        assert (ϵS <~> ϵS') as ϵS_iff_ϵS' by eauto using LR_irrel.
+
         assert (forall s1 s2 ϵs, ϵT s1 s2 ϵs <~> ϵT' s1 s2 (proj1 (ϵS_iff_ϵS' _ _) ϵs)) as ϵT_iff_ϵT'.
-        intros. destruct (H1 _ _ (ϵS_sym _ _ ϵs)) as (_ & K & _).
-        pose (ϵs' := proj1 (ϵS_iff_ϵS' _ _) ϵs).
-        pose (K' := LR_T' _ _ ϵs'). pose proof (L := LR_irrel _ _ _ _ _ _ K K').
-        destruct (H0 _ _ ϵs) as (L' & _). rewrite L'. rewrite L. unfold ϵs'. split; eauto. 
+        { intros. destruct (H1 _ _ (ϵS_sym _ _ ϵs)) as (_ & K & _).
+          pose (ϵs' := proj1 (ϵS_iff_ϵS' _ _) ϵs).
+          pose (K' := LR_T' _ _ ϵs'). pose proof (L := LR_irrel _ _ _ _ _ _ K K').
+          destruct (H0 _ _ ϵs) as (L' & _). rewrite L'. rewrite L. unfold ϵs'. 
+          split; eauto. } 
 
         split.
-        ++ eapply (LR_pi _ _ _ _ _ _ ϵS' _ _ ϵT'); eauto using conv_trans, conv_sym, conv_ty_in_ctx_conv. 
-           eapply LR_S_trans_left in LR_S' as (S1_eq_S' & _). eauto. 
-           intros. pose proof (ϵs' := proj2 (ϵS_iff_ϵS' s1 s2) ϵs).
-           eapply ϵS_sym in ϵs' as ϵs''. 
-           eapply PER_refl in ϵs''.
-           rewrite ϵS_iff_ϵS' in ϵs''.
-           pose (LR_T'' := LR_T' _ _ ϵs'').
-           destruct (H1 _ _ ϵs') as (K & K1 & K2 & K3).
-           unshelve eapply (proj1 (K2 _ _ _)). 2:eauto.
-           eapply LR_iff_rel. 2: apply LR_T''. admit.
-           intros; split; intros; rewrite R'_iff in *.
-           destruct H3. split. admit. 
-           intros. pose (H4' := H4 _ _ ϵs). admit.
-           destruct H3. split. admit.
-           intros. pose (H4' := H4 _ _ ϵs). admit.
+        ++ eapply (LR_pi _ _ _ _ _ _ ϵS' _ _ ϵT'); eauto using conv_trans, conv_sym, conv_ty_in_ctx_conv.
+            +++ eapply LR_S_trans in LR_S' as (S1_eq_S' & _). eauto.
+            +++ intros. pose proof (ϵs' := proj2 (ϵS_iff_ϵS' s1 s2) ϵs).
+                eapply ϵS_sym in ϵs' as ϵs''. 
+                eapply PER_refl in ϵs''; eauto.
+                rewrite ϵS_iff_ϵS' in ϵs''.
+                pose (LR_T'' := LR_T' _ _ ϵs'').
+                destruct (H1 _ _ ϵs') as (K & K1 & K2).
+                unshelve eapply (proj1 (K2 _ _ _)).
+                eapply LR_iff_rel. 2: apply LR_T''. 
+                split; intros ϵT'_t_u;
+                eapply (helper_ϵT_irrel ϵT'); eapply (helper_ϵT_irrel ϵT') in ϵT'_t_u;rewrite <- ϵT_iff_ϵT'; rewrite <- ϵT_iff_ϵT' in ϵT'_t_u.
+                ++++ rewrite (proj2 (H0 _ _ _)). eauto.
+                ++++ rewrite (proj2 (H0 _ _ _)) in ϵT'_t_u. eauto. 
+            +++ intros; split; intros; rewrite R'_iff in *.
+                * destruct H2. split. eauto using conv_conv, conv_pi, conv_sym. 
+                  intros. eapply LR_erasure; eauto. 
+                  ** eapply aconv_app; eauto using conv_sym, conv_ty_in_ctx_conv, LR_escape_tm, type_conv, validity_conv_left, aconv_refl.
+                  ** eapply aconv_conv. 
+                     eapply aconv_app; eauto using validity_conv_right, refl_ty, conv_ty_in_ctx_conv, LR_escape_tm, conv_sym, type_conv.
+                     eapply aconv_conv; eauto using validity_conv_right, aconv_refl, conv_pi.
+                     eauto using conv_aux, LR_escape_tm, conv_sym. Unshelve. eauto. eauto.
+                * destruct H2. split. eauto using conv_conv, conv_pi.
+                intros. eapply LR_erasure; eauto. 
+                ** eapply aconv_conv. 
+                   eapply aconv_app; eauto using LR_escape_tm, validity_conv_left, type_conv, conv_sym, aconv_refl.
+                   eauto 7 using conv_aux, LR_escape_tm, validity_conv_left, type_conv, conv_sym, refl_ty.
+                ** eapply aconv_conv.
+                   eapply aconv_app; eauto using validity_conv_right, refl_ty, conv_sym, conv_ty_in_ctx_conv, LR_escape_tm, type_conv.
+                   eapply aconv_conv; eauto using validity_conv_right, aconv_refl, conv_sym, conv_trans, conv_pi, conv_ty_in_ctx_conv.
+                   eauto using conv_aux, LR_escape_tm, conv_sym, conv_conv.
         ++ intros; split; intro; rewrite H in *; rewrite R'_iff in *.
-           destruct H3. split. admit.
-           intros. pose (H4' := H4 _ _ (proj2 (ϵS_iff_ϵS' _ _) ϵs)). rewrite ϵT_iff_ϵT' in *. admit.
-           destruct H3. split. admit.
-           intros. pose (H4' := H4 _ _ (proj1 (ϵS_iff_ϵS' _ _) ϵs)). rewrite ϵT_iff_ϵT' in *. admit.
-      + admit.
-Admitted.
-           
+            +++ destruct H2. split. eauto using conv_conv, conv_pi. 
+                intros. eapply (helper_ϵT_irrel ϵT'). rewrite <- ϵT_iff_ϵT'. 
+                eapply LR_erasure; eauto.
+                * eapply aconv_app; eauto using LR_escape_tm, validity_conv_left, type_conv, conv_sym, aconv_refl.
+                * eapply aconv_conv.
+                  eapply aconv_app; eauto using LR_escape_tm, validity_conv_right.
+                  eapply aconv_conv; eauto using validity_conv_right, aconv_refl, conv_pi.
+                  eauto 6 using LR_escape_tm, conv_aux, conv_sym, conv_conv. 
+                  Unshelve. apply ϵS_iff_ϵS'. eauto.
+            +++ destruct H2. split. eauto using conv_conv, conv_pi, conv_sym.
+                intros. rewrite ϵT_iff_ϵT'.
+                eapply LR_erasure; eauto.
+                * eapply aconv_app; eauto using conv_sym, conv_ty_in_ctx_conv, LR_escape_tm, validity_conv_left, validity_conv_left, aconv_refl.
+                * eapply aconv_conv.
+                  eapply aconv_app; eauto using conv_sym, conv_ty_in_ctx_conv, LR_escape_tm, validity_conv_right, type_conv.
+                  eapply aconv_conv; eauto using aconv_refl, validity_conv_right, conv_pi.
+                  eauto using conv_aux, conv_sym, LR_escape_tm.
+Qed.
+
+
+Corollary LR_sym l A B R : LR l A B R -> LR l B A R.
+Proof.
+    intros. eapply LR_basic_props in H as (_ & H & _). eauto.
+Qed.
+
+Corollary LR_trans l A B C R : LR l A B R -> LR l B C R -> LR l A C R.
+Proof.
+    intros. eapply LR_basic_props in H as (_ & _ & H). eapply H in H0 as (H1 & H2). eauto.
+Qed.
+
+Corollary LR_sym_tm l A B R t u : LR l A B R -> R t u -> R u t.
+Proof.
+    intros. eapply LR_basic_props in H as ((sym & trans) & _). eauto.
+Qed.
+
+Corollary LR_trans_tm l A B R t u v : LR l A B R -> R t u -> R u v -> R t v.
+Proof.
+    intros. eapply LR_basic_props in H as ((sym & trans) & _). eauto.
+Qed.
+
+
 
 Definition TmLR l t u A := exists B R, LR l A B R /\ R t u.
 
@@ -637,283 +778,6 @@ Lemma LR_conv l A B t u R :
 Proof.
     intros. destruct H0 as (B' & R' & LR & R'_t_u).
     eapply LR_irrel in R'_t_u as R_t_u. 2: apply H. 2:eauto.
-    exists A. exists R. split; auto. admit.
-Admitted.
-
-
-
-(* --- OLD CODE FROM HERE ---
-
-
-
-
-
-Inductive LRTy : forall (k : nat) (rec : forall j, j ◃ (ty k) -> LogRel), LogRel :=
-| LRTy_nat A1 A2 rec : 
-    ∙ ⊢< Ax (ty 0) > A1 ≡ Nat : Sort (ty 0) -> 
-    ∙ ⊢< Ax (ty 0) > A2 ≡ Nat : Sort (ty 0) ->
-    LRTy 0 rec A1 A2 ϵNat
-| LRTy_pi i k rec A1 A2 S1 S2 ϵS T1 T2 ϵT : 
-    ∙ ⊢< Ax (Ru i (ty k)) > A1 ≡ Pi i (ty k) S1 T1 : Sort (Ru i (ty k)) -> 
-    ∙ ⊢< Ax (Ru i (ty k)) > A2 ≡ Pi i (ty k) S2 T2 : Sort (Ru i (ty k)) ->
-    LR_leq (Ru i (ty k)) (LRTy (ru i k) rec) rec i leq_ru_left S1 S2 ϵS -> 
-    (forall s1 s2 (ϵs : ϵS s1 s2), 
-        LR_leq (Ru i (ty k)) (LRTy (ru i k) rec) rec (ty k) leq_ru_right T1 T2 (ϵT s1 s2 ϵs)) ->
-    LRTy (ru i k) rec A1 A2 (ϵPi i (ty k) S1 S2 ϵS T1 T2 ϵT)
-| LRTy_U l A1 A2 rec : 
-    ∙ ⊢< Ax (Ax l) > A1 ≡ Sort l : Sort (Ax l) -> 
-    ∙ ⊢< Ax (Ax l) > A2 ≡ Sort l : Sort (Ax l) ->
-    LRTy (ax l) rec A1 A2 (fun B1 B2 => exists R, rec l lt_ty_ax B1 B2 R).
-(* 
-Scheme LR_leq_mut := Induction for LR_leq Sort Prop
-with LRTy_mut := Induction for LRTy Sort Prop.
-Combined Scheme LR_ty_mutind from LR_leq_mut, LRTy_mut. *)
-
-
-(* Scheme tree_ind' := Induction for LRTy Sort Prop.
-
-
-Scheme list_ind' := Induction for LR_leq Sort Prop.
-Scheme tree_list_ind := Minimality for LRTy Sort Prop
-  with list_ind' := Minimality for LR_leq Sort Prop. *)
-
-Definition LR' (l : level) : LogRel.
-    refine (@well_founded_induction_type _ (fun i j => i ◃ j) _ (fun _ => LogRel) _ l).
-    - apply wf_inverse_image. apply lt_wf.
-    - intros. destruct x.
-        + apply (LRTy n). apply X.
-        + apply LRΩ.
-Defined.
-(* 
-Definition LR (l : level) (p : Acc (λ i j : level, i ◃ j) l): LogRel.
-    refine (@Fix_F _ (fun i j => i ◃ j) (fun _ => LogRel) _ l _).
-    - intros. destruct x.
-        + apply (LRTy n). apply X.
-        + apply LRΩ.
-    - exact p. 
-    (* apply wf_inverse_image. apply lt_wf. *)
-Defined. *)
-
-
-
-Definition LR (l : level) : LogRel.
-    refine (@Fix_F _ (fun i j => i ◃ j) (fun _ => LogRel) _ l _).
-    - intros. destruct x.
-        + apply (LRTy n). apply X.
-        + apply LRΩ.
-    - apply wf_inverse_image. apply lt_wf.
-Defined.
-
-
-Print LR.
-
-Eval compute in (fun i => LR (ty i)).
-
-Axiom proof_irrel : forall (P : Prop) (p q : P), p = q.
-
-Lemma acc_irrel i (f g : forall (l : level) (p : l ◃ ty i), Acc (λ i j : level, i ◃ j) l) : f = g.
-Proof.
-    apply proof_irrel.
+    exists A. exists R. split; auto. eauto using LR_sym.
 Qed.
 
-Lemma LR_prop_eq : LR prop = LRΩ.
-Proof.
-    unfold LR. rewrite <- Fix_F_eq. auto.
-Qed.
-
-Definition nat_to_lvl n := 
-    match n with 
-    | O => prop 
-    | S n => ty n 
-    end.
-
-Lemma lvl_to_nat_to_lvl l : nat_to_lvl (lvl_to_nat l) = l.
-Proof.
-    destruct l.
-    - auto.
-    - auto.
-Qed.
-
-(* Lemma lvl_to_nat_inj *)
-
-Lemma LR_leqeq i j p A B R : LR_leq i (LR i) (fun j _ => LR j) j p A B R <-> LR j A B R.
-Proof.
-    split.
-    - intro H. destruct H.
-        + auto.
-        + rewrite p. auto.
-    - intro H. inversion p.
-        + pose proof (f_equal nat_to_lvl H1). repeat rewrite lvl_to_nat_to_lvl in H0. 
-          eapply LR_leq_eq. eapply proof_irrel. rewrite <- H0. auto. Unshelve. auto. 
-        + assert (lvl_to_nat j < lvl_to_nat i) by lia.
-          eapply LR_leq_lt. eapply proof_irrel. auto. Unshelve. auto.
-Qed.
-
-
-Lemma LR_ty_eq i : 
-    LR (ty i) = LRTy i (fun l _ => LR l).
-Proof.
-    unfold LR. rewrite <- Fix_F_eq. f_equal. 
-(* Set Printing Implicit. *)
-    pattern (fun l => wf_inverse_image level nat lt lvl_to_nat lt_wf l). 
-    set (G := (λ (F : forall l (p : l ◃ ty i), Acc (λ i j : level, i ◃ j) l) (l : level) (p : l ◃ ty i),
-@Fix_F _ (fun x y => x ◃ y) (λ _ : level, LogRel)
-(λ (x : level) (H : ∀ y : level, y ◃ x → LogRel),
-match x as l0 return ((∀ y : level, y ◃ l0 → LogRel) → LogRel) with
-| ty n => λ X : ∀ y : level, y ◃ ty n → LogRel, LRTy n X
-| prop => λ _ : ∀ y : level, y ◃ prop → LogRel, LRΩ
-end H) _ (F l p))).
-    transitivity (G (fun l p => wf_inverse_image level nat lt lvl_to_nat lt_wf l)).
-    erewrite (@acc_irrel i (fun l _ => wf_inverse_image level nat lt lvl_to_nat lt_wf l)). reflexivity. reflexivity.
-Qed.
-
-Definition LR_nat A1 A2 : 
-    ∙ ⊢< Ax (ty 0) > A1 ≡ Nat : Sort (ty 0) -> 
-    ∙ ⊢< Ax (ty 0) > A2 ≡ Nat : Sort (ty 0) ->
-    LR (ty 0) A1 A2 ϵNat.
-Proof.
-    intros. rewrite LR_ty_eq.
-    constructor; eauto.
-Qed.
-
-Definition LR_U l A1 A2 : 
-    ∙ ⊢< Ax (Ax l) > A1 ≡ Sort l : Sort (Ax l) -> 
-    ∙ ⊢< Ax (Ax l) > A2 ≡ Sort l : Sort (Ax l) ->
-    LR (Ax l) A1 A2 (fun B1 B2 => exists R, LR l B1 B2 R).
-Proof.
-    intros. unfold Ax. rewrite LR_ty_eq.
-    constructor; eauto.
-Qed.
-
-Definition LR_pi i k A1 A2 S1 S2 ϵS T1 T2 ϵT : 
-    ∙ ⊢< Ax (Ru i (ty k)) > A1 ≡ Pi i (ty k) S1 T1 : Sort (Ru i (ty k)) -> 
-    ∙ ⊢< Ax (Ru i (ty k)) > A2 ≡ Pi i (ty k) S2 T2 : Sort (Ru i (ty k)) ->
-    LR i S1 S2 ϵS -> 
-    (forall s1 s2 (ϵs : ϵS s1 s2), LR (ty k) T1 T2 (ϵT s1 s2 ϵs)) ->
-    LR (Ru i (ty k)) A1 A2 (ϵPi i (ty k) S1 S2 ϵS T1 T2 ϵT).
-Proof.
-    intros. unfold Ru. rewrite LR_ty_eq.
-    constructor; eauto.
-    - rewrite <- LR_ty_eq. rewrite LR_leqeq. auto.
-    - rewrite <- LR_ty_eq. setoid_rewrite LR_leqeq. auto.
-Qed.
-
-
-Definition LR_ind 
-    (P : forall l A B R, Prop)
-    (p_prop : forall A B R (p : LRΩ A B R), P prop A B R) 
-    (p_nat : forall A1 A2
-        (A1_red_nat : ∙ ⊢< Ax (ty 0) > A1 ≡ Nat : Sort (ty 0))
-        (A2_red_nat : ∙ ⊢< Ax (ty 0) > A2 ≡ Nat : Sort (ty 0)),
-        P (ty 0) A1 A2 ϵNat)
-    (p_U : forall l A1 A2
-        (A1_red_U : ∙ ⊢< Ax (Ax l) > A1 ≡ Sort l : Sort (Ax l))
-        (A2_red_U : ∙ ⊢< Ax (Ax l) > A2 ≡ Sort l : Sort (Ax l)),
-        P (Ax l) A1 A2 (fun B1 B2 => exists R, LR l B1 B2 R))
-    (p_pi : forall i k A1 A2 S1 S2 ϵS T1 T2 ϵT
-        (A1_red_pi : ∙ ⊢< Ax (Ru i (ty k)) > A1 ≡ Pi i (ty k) S1 T1 : Sort (Ru i (ty k)))
-        (A2_red_pi : ∙ ⊢< Ax (Ru i (ty k)) > A2 ≡ Pi i (ty k) S2 T2 : Sort (Ru i (ty k)))
-        (LR_S : LR i S1 S2 ϵS)
-        (LR_T : forall s1 s2 (ϵs : ϵS s1 s2), 
-                LR (ty k) T1 T2 (ϵT s1 s2 ϵs)),
-        P i S1 S2 ϵS -> 
-        (forall s1 s2 (ϵs : ϵS s1 s2), P (ty k) T1 T2 (ϵT s1 s2 ϵs)) ->
-        P (Ru i (ty k)) A1 A2 (ϵPi i (ty k) S1 S2 ϵS T1 T2 ϵT))
-    (l : level) (A B : term) (R : TmRel) (x : LR l A B R) : P l A B R.
-Proof.
-    destruct l.
-    - rewrite LR_ty_eq in x. 
-      set (rec := (λ (l : level) (_ : l ◃ ty n), LR l)).
-        assert (rec = (λ (l : level) (_ : l ◃ ty n), LR l)) by reflexivity.
-        rewrite <- H in x.
-        generalize n rec H A B R x.
-        clear n rec H A B R x.
-        fix IH 1. intros.
-        destruct x.
-        + apply p_nat; auto.
-        + 
-        (* pose proof H2 as H2'. pose proof H3 as H3'. *)
-          (* rewrite H in H2, H3.
-          rewrite <- LR_ty_eq in H2,H3.
-          rewrite LR_leqeq in H2.
-          setoid_rewrite LR_leqeq in H3. *)
-          apply p_pi; auto.
-          ++ rewrite H in H2. rewrite <- LR_ty_eq in H2. rewrite LR_leqeq in H2. auto.
-          ++ rewrite H in H3. rewrite <- LR_ty_eq in H3. setoid_rewrite LR_leqeq in H3. auto.
-          ++ destruct i. 
-           +++ eapply IH; auto. reflexivity. destruct H2. 
-           
-           rewrite H in H2. rewrite <- LR_ty_eq in H2. rewrite LR_leqeq in H2. rewrite <- LR_ty_eq. auto.
-           +++ rewrite H in H2. rewrite <- LR_ty_eq in H2. rewrite LR_leqeq in H2. apply p_prop. rewrite LR_prop_eq in H2. apply H2.
-          ++ intros. eapply IH; eauto. reflexivity. 
-             rewrite H in H3. rewrite <- LR_ty_eq in H3. setoid_rewrite LR_leqeq in H3. 
-             rewrite <- LR_ty_eq. apply H3.
-          (* ++ intros. apply LR_ind; auto. *)
-        + rewrite H. apply p_U; auto.
-    - rewrite LR_prop_eq in x. apply p_prop. auto.
-Qed.
-
-Lemma LR_ind 
-    (P : forall l A B R, LR l A B R -> Prop)
-    (p_prop : forall A B R p, P prop A B R p) 
-    (p_nat : forall A1 A2
-        (A1_red_nat : ∙ ⊢< Ax (ty 0) > A1 ≡ Nat : Sort (ty 0))
-        (A2_red_nat : ∙ ⊢< Ax (ty 0) > A2 ≡ Nat : Sort (ty 0)),
-        P _ _ _ _ (LR_nat A1 A2 A1_red_nat A2_red_nat))
-    (p_U : forall l A1 A2
-        (A1_red_U : ∙ ⊢< Ax (Ax l) > A1 ≡ Sort l : Sort (Ax l))
-        (A2_red_U : ∙ ⊢< Ax (Ax l) > A2 ≡ Sort l : Sort (Ax l)),
-        P _ _ _ _ (LR_U l A1 A2 A1_red_U A2_red_U))
-    (p_pi : forall i k A1 A2 S1 S2 ϵS T1 T2 ϵT
-        (A1_red_pi : ∙ ⊢< Ax (Ru i (ty k)) > A1 ≡ Pi i (ty k) S1 T1 : Sort (Ru i (ty k)))
-        (A2_red_pi : ∙ ⊢< Ax (Ru i (ty k)) > A2 ≡ Pi i (ty k) S2 T2 : Sort (Ru i (ty k)))
-        (LR_S : LR i S1 S2 ϵS)
-        (LR_T : forall s1 s2 (ϵs : ϵS s1 s2), 
-                LR (ty k) T1 T2 (ϵT s1 s2 ϵs)),
-        P _ _ _ _ LR_S -> 
-        (forall s1 s2 (ϵs : ϵS s1 s2), P _ _ _ _ (LR_T s1 s2 ϵs)) ->
-        P _ _ _ _ (LR_pi i k A1 A2 S1 S2 ϵS T1 T2 ϵT A1_red_pi A2_red_pi LR_S LR_T))
-    (l : level) (A B : term) (R : TmRel) (x : LR l A B R) : P _ _ _ _ x.
-Proof.
-    destruct l.
-    - pose proof x as x'. rewrite LR_ty_eq in x'. induction x'.
-    + 
-    - apply p_prop.
-
-            
-Lemma LR_irrel l A B R1 R2 : 
-    LR l A B R1 -> 
-    LR l A B R2 -> 
-    forall t1 t2, R1 t1 t2 <-> R2 t1 t2.
-Proof.
-    intros LR1 LR2.
-    induction l.
-    - rewrite LR_ty_eq in *. 
-        set (rec := (λ (l : level) (_ : l ◃ ty n), LR l)).
-        assert (rec = (λ (l : level) (_ : l ◃ ty n), LR l)) by reflexivity.
-        rewrite <- H in LR1, LR2.
-    induction LR1. admit. 
-    repeat rewrite H in H2. rewrite <- LR_ty_eq in H2. rewrite LR_leqeq in H2. 
-    repeat rewrite H in H3. rewrite <- LR_ty_eq in H3.
-    setoid_rewrite LR_leqeq in H3.
-    induction LR2.
-    admit.
-    rewrite H in *. rewrite <- LR_ty_eq in *. rewrite LR_leqeq in *.
-    setoid_rewrite LR_leqeq in H7.
-
-        admit. admit. admit.
-        rewrite <- LR_ty_eq  in H1.
-        setoid_rewrite LR_leqeq in H1. 
-        rewrite <- LR_ty_eq in H2.
-        setoid_rewrite LR_leqeq in H2.
-        
-        admit.
-        rewrite <- LR_ty_eq  in H1, H2.
-        setoid_rewrite LR_leqeq in H1. 
-        setoid_rewrite LR_leqeq in H2.    
-        
-        fold LR in *.  admit. all:admit.
-    - rewrite LR_prop_eq in *. destruct LR1 as (_ & equiv1). destruct LR2 as (_ & equiv2).
-        intros. split; setoid_rewrite equiv1; setoid_rewrite equiv2; auto.
-Admitted.
- *)
